Phi_Examples/Binary_Search.thy
@@ -11,7 +11,7 @@ proc binary_search_array:
           (LEAST i. lower \<le> i \<and> i \<le> upper \<and> arr!i \<le> k) \<Ztypecolon> \<v>\<a>\<l> \<nat>(\<i>\<n>\<t>)\<close>
   is [routine]
 \<medium_left_bracket>
-  if ($ptr \<tribullet> $lower! \<le> $k) \<medium_left_bracket>
+  if ($ptr.$lower! \<le> $k) \<medium_left_bracket>
     return ($lower)
   \<medium_right_bracket> \<medium_left_bracket>
     ($lower, $upper) \<rightarrow> var $l, $u
