Phi_Examples/Dynamic_Array.thy
@@ -4,7 +4,7 @@ theory Dynamic_Array
           PhiStd.PhiStd_Slice
 begin
 
-\<phi>type_def DynArr :: \<open>logaddr \<Rightarrow> TY \<Rightarrow> (VAL, 'x) \<phi> \<Rightarrow> (fiction, 'x list) \<phi>\<close>
+\<phi>type_def DynArr :: \<open>address \<Rightarrow> TY \<Rightarrow> (VAL, 'x) \<phi> \<Rightarrow> (fiction, 'x list) \<phi>\<close>
   where \<open>l \<Ztypecolon> DynArr addr TY T \<equiv> (a\<^sub>D, len, cap) \<Ztypecolon> \<m>\<e>\<m>[addr] \<lbrace> data: \<bbbP>\<t>\<r> \<a>\<r>\<r>\<a>\<y>[cap] TY, len: \<nat>(\<s>\<i>\<z>\<e>_\<t>), cap: \<nat>(\<s>\<i>\<z>\<e>_\<t>) \<rbrace>\<heavy_comma>
                                 data \<Ztypecolon> \<m>\<e>\<m>[a\<^sub>D] \<bbbA>\<r>\<r>\<a>\<y>[cap] T
                                 \<s>\<u>\<b>\<j> a\<^sub>D len cap data. len = length l \<and> cap = length data \<and>
