Phi_Examples/Matrix_Oprs.thy
@@ -7,7 +7,7 @@ begin
 
 abbreviation \<open>\<m>\<a>\<t> M N \<equiv> \<a>\<r>\<r>\<a>\<y>[M] \<a>\<r>\<r>\<a>\<y>[N] \<i>\<n>\<t>\<close>
 
-\<phi>type_def MatSlice :: \<open>logaddr \<Rightarrow> nat \<Rightarrow> nat \<Rightarrow> nat \<Rightarrow> nat \<Rightarrow> (fiction, int mat) \<phi>\<close>
+\<phi>type_def MatSlice :: \<open>address \<Rightarrow> nat \<Rightarrow> nat \<Rightarrow> nat \<Rightarrow> nat \<Rightarrow> (fiction, int mat) \<phi>\<close>
   where \<open>x \<Ztypecolon> MatSlice addr i j m n \<equiv> l \<Ztypecolon> \<m>\<e>\<m>[addr] \<s>\<l>\<i>\<c>\<e>[i,m] (\<s>\<l>\<i>\<c>\<e>[j,n] \<int>\<^sup>r(\<i>\<n>\<t>))
                                      \<s>\<u>\<b>\<j> l. l = mat_to_list x \<and> x \<in> carrier_mat m n\<close>
 
@@ -29,7 +29,7 @@ proc zero_mat:
 \<medium_left_bracket>
   map_slice ($m) \<medium_left_bracket> for k \<rightarrow> val k \<semicolon>
     map_slice ($n) \<medium_left_bracket> for h \<rightarrow> val h \<semicolon>
-      $a \<tribullet> ($i + $k) \<tribullet> ($j + $h) := \<open>0 \<Ztypecolon> \<int>\<^sup>r(\<i>\<n>\<t>)\<close>
+      $a[$i + $k, $j + $h] := \<open>0 \<Ztypecolon> \<int>\<^sup>r(\<i>\<n>\<t>)\<close>
     \<medium_right_bracket>
   \<medium_right_bracket> \<semicolon>
 
@@ -75,7 +75,7 @@ proc copy_mat:
 \<medium_left_bracket>
   map_2slice ($m) \<medium_left_bracket> for k \<rightarrow> val k \<semicolon>
     map_2slice ($n) \<medium_left_bracket> for h \<rightarrow> val h \<semicolon>
-      $a\<^sub>x \<tribullet> ($i\<^sub>x + $k) \<tribullet> ($j\<^sub>x + $h) := $a\<^sub>y \<tribullet> ($i\<^sub>y + $k) \<tribullet> ($j\<^sub>y + $h ) !
+      $a\<^sub>x[$i\<^sub>x + $k, $j\<^sub>x + $h] := $a\<^sub>y[$i\<^sub>y + $k, $j\<^sub>y + $h] !
     \<medium_right_bracket> \<semicolon>
   \<medium_right_bracket>
 \<medium_right_bracket> .
@@ -97,7 +97,7 @@ proc add_mat:
 \<medium_left_bracket>
   map_2slice ($m) \<medium_left_bracket> for k \<rightarrow> val k
     map_2slice ($n) \<medium_left_bracket> for h \<rightarrow> val h
-        $a\<^sub>x \<tribullet> ($i\<^sub>x + $k) \<tribullet> ($j\<^sub>x + $h) := $a\<^sub>x \<tribullet> ($i\<^sub>x + $k) \<tribullet> ($j\<^sub>x + $h) ! + $a\<^sub>y \<tribullet> ($i\<^sub>y + $k) \<tribullet> ($j\<^sub>y + $h ) !
+        $a\<^sub>x[$i\<^sub>x + $k, $j\<^sub>x + $h] := $a\<^sub>x[$i\<^sub>x + $k, $j\<^sub>x + $h]! + $a\<^sub>y[$i\<^sub>y + $k, $j\<^sub>y + $h]!
     \<medium_right_bracket> \<semicolon>
   \<medium_right_bracket>
 \<medium_right_bracket> .
@@ -119,7 +119,7 @@ proc sub_mat:
 \<medium_left_bracket>
   map_2slice ($m) \<medium_left_bracket> for k \<rightarrow> val k \<semicolon>
     map_2slice ($n) \<medium_left_bracket> for h \<rightarrow> val h \<semicolon>
-      $a\<^sub>x \<tribullet> ($i\<^sub>x + $k) \<tribullet> ($j\<^sub>x + $h) := $a\<^sub>x \<tribullet> ($i\<^sub>x + $k) \<tribullet> ($j\<^sub>x + $h) ! - $a\<^sub>y \<tribullet> ($i\<^sub>y + $k) \<tribullet> ($j\<^sub>y + $h ) ! 
+      $a\<^sub>x[$i\<^sub>x + $k, $j\<^sub>x + $h] := $a\<^sub>x[$i\<^sub>x + $k, $j\<^sub>x + $h]! - $a\<^sub>y[$i\<^sub>y + $k, $j\<^sub>y + $h]! 
     \<medium_right_bracket> \<semicolon>
   \<medium_right_bracket> \<semicolon>
 \<medium_right_bracket> .
@@ -184,7 +184,7 @@ proc strassen:
     \<open>MatSlice a\<^sub>A _ _ _ _\<close> \<t>\<r>\<a>\<n>\<s>\<f>\<o>\<r>\<m>\<s>_\<t>\<o> \<o>\<p>\<e>\<n>
     \<open>MatSlice a\<^sub>B _ _ _ _\<close> \<t>\<r>\<a>\<n>\<s>\<f>\<o>\<r>\<m>\<s>_\<t>\<o> \<o>\<p>\<e>\<n> \<semicolon>
 
-    $a\<^sub>A \<tribullet> $i\<^sub>A \<tribullet> $j\<^sub>A := $a\<^sub>A \<tribullet> $i\<^sub>A \<tribullet> $j\<^sub>A ! * $a\<^sub>B \<tribullet> $i\<^sub>B \<tribullet> $j\<^sub>B ! \<semicolon>
+    $a\<^sub>A[$i\<^sub>A, $j\<^sub>A] := $a\<^sub>A[$i\<^sub>A, $j\<^sub>A]! * $a\<^sub>B[$i\<^sub>B, $j\<^sub>B]! \<semicolon>
       
     holds_fact [\<phi>sledgehammer_simps]: \<open>dim_col B = 1 \<and> dim_row B = 1 \<and> dim_col A = 1 \<and> dim_row A = 1\<close> (*for proof obligation*)
     note scalar_prod_def [\<phi>sledgehammer_simps] \<semicolon>                                       (*for proof obligation*)
