Phi_System/Calculus_of_Programming.thy
@@ -45,14 +45,14 @@ consts programming_mode :: mode
 definition CurrentConstruction :: " mode \<Rightarrow> resource \<Rightarrow> assn \<Rightarrow> assn \<Rightarrow> bool "
   where "CurrentConstruction mode s R S \<longleftrightarrow> s \<in> INTERP_SPEC (S * R)"
 
-abbreviation Programming_CurrentConstruction ("\<c>\<u>\<r>\<r>\<e>\<n>\<t> _ [_]/ \<r>\<e>\<s>\<u>\<l>\<t>\<s> \<i>\<n> _" [1000,1000,11] 10)
+abbreviation Programming_CurrentConstruction ("(2\<c>\<u>\<r>\<r>\<e>\<n>\<t> _ [_] \<r>\<e>\<s>\<u>\<l>\<t>\<s> \<i>\<n>/ _)" [1000,1000,11] 10)
   where \<open>Programming_CurrentConstruction \<equiv> CurrentConstruction programming_mode\<close>
 
-abbreviation View_Shift_CurrentConstruction ("\<v>\<i>\<e>\<w> _ [_]/ \<i>\<s> _" [1000,1000,11] 10)
+abbreviation View_Shift_CurrentConstruction ("(2\<v>\<i>\<e>\<w> _ [_] \<i>\<s>/ _)" [1000,1000,11] 10)
   where \<open>View_Shift_CurrentConstruction \<equiv> CurrentConstruction view_shift_mode\<close>
 
-consts Programming_CurrentConstruction_syntax :: \<open>assn \<Rightarrow> bool\<close> ("\<c>\<u>\<r>\<r>\<e>\<n>\<t> \<s>\<t>\<a>\<t>\<e>: _" [11] 10)
-consts View_Shift_CurrentConstruction_syntax :: \<open>assn \<Rightarrow> bool\<close> ("\<c>\<u>\<r>\<r>\<e>\<n>\<t> \<v>\<i>\<e>\<w>: _" [11] 10)
+consts Programming_CurrentConstruction_syntax :: \<open>assn \<Rightarrow> bool\<close> ("(2\<c>\<u>\<r>\<r>\<e>\<n>\<t> \<s>\<t>\<a>\<t>\<e>:/ _)" [11] 10)
+consts View_Shift_CurrentConstruction_syntax :: \<open>assn \<Rightarrow> bool\<close> ("(2\<c>\<u>\<r>\<r>\<e>\<n>\<t> \<v>\<i>\<e>\<w>:/ _)" [11] 10)
 
 definition PendingConstruction :: " 'ret proc
                                   \<Rightarrow> resource
